KeyManagement/Simulation.v
@@ -159,19 +159,80 @@ Section SingleAdversarySimulates.
    *   or, prove an appended simulation relation, but I am not sure how to generically express this
    *)
 
-  Definition ADV := 10.
+  Section AdversaryHelpers.
+    Import RealWorld.
 
-  Definition add_adversary {A B} (U__r : RealWorld.universe A B) (advcode : RealWorld.user_cmd B) :=
-    RealWorld.addAdversaries U__r ($0 $+ (ADV, {| RealWorld.key_heap := $0
-                                              ; RealWorld.msg_heap := []
-                                              ; RealWorld.protocol := advcode |})).
+    Definition ADV := 10.
 
-  Definition strip_adversary {A B} (U__r : RealWorld.universe A B) : RealWorld.universe A B :=
-    {| RealWorld.users       := U__r.(RealWorld.users)
-     ; RealWorld.adversary   := $0
-     ; RealWorld.all_ciphers := U__r.(RealWorld.all_ciphers)
-     |}.
+    Definition add_adversary {A B} (U__r : universe A B) (advcode : user_cmd B) :=
+      addAdversaries U__r ($0 $+ (ADV, {| key_heap := $0
+                                      ; msg_heap := []
+                                      ; protocol := advcode |})).
 
+    Fixpoint msg_safe {t} (msg : message t) : bool :=
+      match msg with
+      | Plaintext _ => false
+      | KeyMessage _ => false
+      | MsgPair m1 m2 => msg_safe m1 && msg_safe m2
+      | Ciphertext _ => true
+      | Signature _ _ => true
+      end.
+
+    Definition exm_safe (msg : exmsg) : bool :=
+      match msg with
+      | Exm m => true
+      end.
+
+    Definition clean_messages (msgs : queued_messages) :=
+      List.filter exm_safe msgs.
+
+    Definition clean_users {A} ( usrs : honest_users A ) :=
+      map (fun u_d => {| key_heap := u_d.(key_heap)
+                    ; protocol := u_d.(protocol)
+                    ; msg_heap := clean_messages u_d.(msg_heap) |}) usrs.
+
+    Definition honest_cipher (adv_keys : keys) (c : cipher) :=
+      match c with
+      | Cipher _ k_id _ =>
+        match adv_keys $? k_id with
+        | Some (SymKey _) => false
+        | Some (AsymKey _ true) => false
+        | _ => true
+        end
+      end.
+
+    Definition clean_ciphers (adv_keys : keys) (cs : ciphers) :=
+      fold (fun k v m => if honest_cipher adv_keys v then m $+ (k,v) else m) cs $0.
+
+    Definition strip_adversary {A B} (U__r : universe A B) : universe A B :=
+      {| users       := U__r.(users)
+       ; adversary   := $0
+       ; all_ciphers := clean_ciphers (findUserKeys U__r.(adversary)) U__r.(all_ciphers)
+      |}.
+
+    Lemma cipher_is_Cipher :
+      forall v : cipher,
+        match v with
+        | RealWorld.Cipher _ _ _ => true
+        end = true.
+    Proof.
+      destruct v; auto.
+    Qed.
+
+    Lemma clean_ciphers_nokeys_idempotent :
+      forall cs,
+        clean_ciphers $0 cs = cs.
+    Proof.
+      intros.
+      unfold clean_ciphers, honest_cipher.
+      simpl.
+
+      (* rewrite cipher_is_Cipher. *)
+      admit.
+
+    Admitted.
+
+  End AdversaryHelpers.
 
   Section RealWorldLemmas.
     Import RealWorld.
@@ -200,18 +261,314 @@ Section SingleAdversarySimulates.
       eexists; intuition. eassumption.
     Qed.
 
+    (* Lemma honest_step_advuniv_implies_honest_step_origuniv : *)
+    (*   forall {A B C} cs cs' lbl u_id (usrs usrs' : honest_users A) (adv adv' : adversaries B) ks ks' qmsgs qmsgs' bd bd', *)
+    (*     step_user u_id lbl bd bd' *)
+    (*     -> forall (cmd : user_cmd C), *)
+    (*       bd = (usrs, adv, cs, ks, qmsgs, cmd) *)
+    (*       -> forall cmd', *)
+    (*         bd' = (usrs', adv', cs', ks', qmsgs', cmd') *)
+    (*         -> step_user (B:=B) u_id lbl (usrs, $0, cs, ks, qmsgs, cmd) (usrs', $0, cs', ks', qmsgs', cmd'). *)
+    (* Proof. *)
+    (*   induction 1; inversion 1; inversion 1; subst; econstructor; eauto. *)
+    (*   unfold addUserKeys; m_equal; trivial. *)
+    (* Qed. *)
+
+    (* Print data_step0. *)
+
     Lemma honest_step_advuniv_implies_honest_step_origuniv :
+      forall {A B C} cs cs' lbl u_id (usrs usrs' : honest_users A) (adv adv' : adversaries B) ks ks' qmsgs qmsgs' bd bd',
+        step_user u_id lbl bd bd'
+        -> forall (cmd : user_cmd C) cs__s adv_keys,
+          adv_keys = findUserKeys adv
+          -> cs__s = clean_ciphers adv_keys cs
+          -> bd = (usrs, adv, cs, ks, qmsgs, cmd)
+          -> forall cmd' cs__s',
+              cs__s' = clean_ciphers adv_keys cs'
+              -> bd' = (usrs', adv', cs', ks', qmsgs', cmd')
+              -> step_user (B:=B) u_id lbl (usrs, $0, cs__s, ks, qmsgs, cmd) (usrs', $0, cs__s', ks', qmsgs', cmd').
+    Proof.
+      induction 1; inversion 3; inversion 2; subst.
+      - econstructor; eauto.
+      - econstructor; eauto.
+      - econstructor; eauto.
+      -
+        (* eapply StepRecv. *)
+
+  (* H3 : msg_accepted_by_pattern cs' pat msg = true *)
+  (* ============================ *)
+  (* step_user u_id (Action (Input msg pat u_id ks cs')) (usrs', $0, clean_ciphers (findUserKeys adv') cs', ks, Exm msg :: qmsgs', Recv pat) *)
+  (*   (usrs', $0, clean_ciphers (findUserKeys adv') cs', ks $++ findKeys msg, qmsgs', Return msg) *)
+        admit.
+
+      - econstructor; eauto.
+
+        (* H1 : msg_accepted_by_pattern cs' pat msg = false *)
+        (* ============================ *)
+        (* msg_accepted_by_pattern (clean_ciphers (findUserKeys adv') cs') pat msg = false *)
+
+        admit.
+
+      - econstructor; eauto; unfold addUserKeys; m_equal; trivial.
+      - econstructor; eauto.
+
+      (* Two goals: *)
+
+      (* H0 : ks' $? keyId k = Some k *)
+      (* H1 : ~ In (elt:=cipher) c_id cs *)
+      (* H2 : encryptMessage k msg c_id = Some cipherMsg *)
+      (* ============================ *)
+      (* ~ In (elt:=cipher) c_id (clean_ciphers (findUserKeys adv') cs) *)
+        admit.
+
+      (* H0 : ks' $? keyId k = Some k *)
+      (* H1 : ~ In (elt:=cipher) c_id cs *)
+      (* H2 : encryptMessage k msg c_id = Some cipherMsg *)
+      (* ============================ *)
+      (* clean_ciphers (findUserKeys adv') (cs $+ (c_id, cipherMsg)) = clean_ciphers (findUserKeys adv') cs $+ (c_id, cipherMsg) *)
+        admit.
+
+      - econstructor; eauto.
+
+      (* H0 : ks $? key_id k = Some (AsymKey k true) \/ ks $? key_id k = Some (SymKey k) *)
+      (* H6 : (usrs', adv', cs', ks, qmsgs', Decrypt (Ciphertext c_id)) = (usrs', adv', cs', ks, qmsgs', Decrypt (Ciphertext c_id)) *)
+      (* H : cs' $? c_id = Some (Cipher c_id (key_id k) msg) *)
+      (* ============================ *)
+      (* clean_ciphers (findUserKeys adv') cs' $? c_id = Some (Cipher c_id (key_id k) msg) *)
+        admit.
+
+      - econstructor; eauto.
+
+      (* H0 : ks' $? keyId k = Some k *)
+      (* H1 : ~ In (elt:=cipher) c_id cs *)
+      (* H2 : signMessage k msg c_id = Some cipherMsg *)
+      (* H6 : (usrs', adv', cs, ks', qmsgs', Sign k msg) = (usrs', adv', cs, ks', qmsgs', Sign k msg) *)
+      (* ============================ *)
+      (* ~ In (elt:=cipher) c_id (clean_ciphers (findUserKeys adv') cs) *)
+        admit.
+
+      (* H0 : ks' $? keyId k = Some k *)
+      (* H1 : ~ In (elt:=cipher) c_id cs *)
+      (* H2 : signMessage k msg c_id = Some cipherMsg *)
+      (* H6 : (usrs', adv', cs, ks', qmsgs', Sign k msg) = (usrs', adv', cs, ks', qmsgs', Sign k msg) *)
+      (* ============================ *)
+      (* clean_ciphers (findUserKeys adv') (cs $+ (c_id, cipherMsg)) = clean_ciphers (findUserKeys adv') cs $+ (c_id, cipherMsg) *)
+        admit.
+
+      - econstructor; eauto.
+
+        (* H : ks' $? keyId k = Some k *)
+        (* H0 : cs' $? c_id = Some (Cipher c_id k_id msg) *)
+        (* ============================ *)
+        (* clean_ciphers (findUserKeys adv') cs' $? c_id = Some (Cipher c_id k_id msg) *)
+        admit.
+    Admitted.
+
+    Lemma enc_cipher_has_key :
+      forall {t} k (msg : message t) c_id cipherMsg,
+        encryptMessage k msg c_id = Some cipherMsg
+        -> cipherMsg = Cipher c_id (keyId k) msg
+        /\ (exists cryp_key, k = SymKey cryp_key \/ k = AsymKey cryp_key false).
+    Proof.
+      intros.
+      unfold encryptMessage in H.
+      case_eq k; intros; rewrite H0 in H.
+      - case_eq (usage k0); intro; rewrite H1 in H; invert H; eauto.
+      - case_eq has_private_access; intro; rewrite H1 in H;
+          case_eq (usage k0); intro; rewrite H2 in H || invert H; invert H; eauto.
+    Qed.
+
+    Lemma sign_cipher_has_key :
+      forall {t} k (msg : message t) c_id cipherMsg,
+        signMessage k msg c_id = Some cipherMsg
+        -> cipherMsg = Cipher c_id (keyId k) msg
+          /\ (exists cryp_key, k = SymKey cryp_key \/ k = AsymKey cryp_key true).
+    Proof.
+      intros.
+      unfold signMessage in H.
+
+      case_eq k; intros; rewrite H0 in H.
+      - case_eq (usage k0); intro; rewrite H1 in H; invert H; eauto.
+      - case_eq has_private_access; intro; rewrite H1 in H;
+          case_eq (usage k0); intro; rewrite H2 in H || invert H; invert H; eauto.
+    Qed.
+
+    Lemma honest_cipher_proper_morphism :
+      forall ks,
+        Morphisms.Proper (Morphisms.respectful eq (Morphisms.respectful eq (Morphisms.respectful eq eq)))
+                         (fun (k : NatMap.key) (c : cipher) (cs : t cipher) => if honest_cipher ks c then cs $+ (k, c) else cs).
+    Proof.
+      unfold Morphisms.Proper, Morphisms.respectful; simpl. intros. subst. simpl.
+      case (honest_cipher ks y0); eauto.
+    Qed.
+
+    Lemma honest_cipher_transpose_key :
+      forall ks,
+        transpose_neqkey eq (fun (k : NatMap.key) (c : cipher) (cs : t cipher) => if honest_cipher ks c then cs $+ (k, c) else cs).
+    Proof.
+      unfold transpose_neqkey; simpl.
+      intros.
+      case (honest_cipher ks e); eauto.
+      case (honest_cipher ks e'); eauto.
+      apply map_eq_Equal; unfold Equal; intros.
+      case (y ==n k); intro; subst.
+      - rewrite add_eq_o by trivial. rewrite add_neq_o by auto. rewrite add_eq_o by trivial. auto.
+      - rewrite add_neq_o by auto.
+        case (y ==n k'); intros; subst.
+        do 2 rewrite add_eq_o by trivial. trivial.
+        do 3 rewrite add_neq_o by auto. trivial.
+    Qed.
+
+    Hint Resolve honest_cipher_proper_morphism honest_cipher_transpose_key.
+
+    (* Specialize to single adversary.  This means that in the following proof, we assume
+     * that, since we are stepping the adversary, then
+     *   ks =  adv keys at beginning
+     *   ks' = adv keys at the end
+     *)
+    Lemma adv_step_implies_no_new_ciphers_after_cleaning :
+      forall {A B C} cs cs' lbl u_id (usrs usrs' : honest_users A) (adv adv' : adversaries B) ks ks' qmsgs qmsgs' bd bd',
+        step_user u_id lbl bd bd'
+        -> forall (cmd : user_cmd C) cs__s,
+            bd = (usrs, adv, cs, ks, qmsgs, cmd)
+          -> cs__s = clean_ciphers ks cs
+          (* -> (forall k_id v, MapsTo k_id v ks -> MapsTo k_id v adv_keys) *)
+          -> forall cmd' cs__s',
+                bd' = (usrs', adv', cs', ks', qmsgs', cmd')
+              -> cs__s' = clean_ciphers ks' cs'
+              -> cs__s = cs__s'.
+    Proof.
+      induction 1; inversion 1; inversion 2; subst; eauto.
+
+      - admit.
+
+      -  admit.
+         
+      -  admit.
+
+      - intros; subst.
+        unfold clean_ciphers; simpl.
+        rewrite fold_add; simpl; eauto.
+
+        assert (honest_cipher ks' cipherMsg = false).
+        apply sign_cipher_has_key in H2; invert H2; subst; simpl.
+        invert H3. rewrite H0. invert H; eauto.
+        rewrite H; trivial.
+
+    Admitted.
+
+    Lemma user_step_adds_no_users :
       forall {A B C} cs cs' lbl u_id (usrs usrs' : honest_users A) (adv adv' : adversaries B) ks ks' qmsgs qmsgs' bd bd',
         step_user u_id lbl bd bd'
         -> forall (cmd : user_cmd C),
           bd = (usrs, adv, cs, ks, qmsgs, cmd)
           -> forall cmd',
             bd' = (usrs', adv', cs', ks', qmsgs', cmd')
-            -> step_user (B:=B) u_id lbl (usrs, $0, cs, ks, qmsgs, cmd) (usrs', $0, cs', ks', qmsgs', cmd').
+            -> forall u_id' u_d,
+              usrs' $? u_id' = Some u_d
+              -> usrs $? u_id' <> None.
     Proof.
-      induction 1; inversion 1; inversion 1; subst; econstructor; eauto.
-      unfold addUserKeys; m_equal; trivial.
+      induction 1; inversion 1; inversion 1; intros; subst; eauto;
+        repeat match goal with
+               | [ H : ?us $? ?uid = Some _ |- ?us $? ?uid <> None ] => solve [ rewrite H; intro C; invert C ]
+               end.
+
+      case (u_id' ==n rec_u_id); intro.
+      - subst. rewrite H1; intro C; invert C.
+      - rewrite add_neq_o in H11 by auto.
+        rewrite H11; intro C; invert C.
     Qed.
+
+    Lemma user_step_adds_removes_no_adversaries :
+      forall {A B C} cs cs' lbl u_id (usrs usrs' : honest_users A) (adv adv' : adversaries B) ks ks' qmsgs qmsgs' bd bd',
+        step_user u_id lbl bd bd'
+        -> forall (cmd : user_cmd C),
+          bd = (usrs, adv, cs, ks, qmsgs, cmd)
+          -> forall cmd',
+            bd' = (usrs', adv', cs', ks', qmsgs', cmd')
+            -> (forall u_id',
+                  adv' $? u_id' <> None
+                  <-> adv $? u_id' <> None).
+    Proof.
+      induction 1; inversion 1; inversion 1; intros; subst; eauto;
+        unfold iff; constructor; intro; eauto.
+
+      - unfold addUserKeys in H. rewrite <- in_find_iff in H.
+        rewrite map_in_iff in H. apply in_find_iff; eauto.
+
+      - unfold addUserKeys; apply in_find_iff.
+        rewrite <- in_find_iff in H.
+        rewrite map_in_iff; eauto.
+    Qed.
+
+
+    (* Lemma universe_step_adds_no_users : *)
+    (*   forall {A B} (U U' : universe A B) lbl, *)
+    (*     step_universe U lbl U' *)
+    (*     -> forall u_id u_d, *)
+    (*       U'.(users) $? u_id = Some u_d -> U.(users) $? u_id <> None. *)
+    (* Proof. *)
+    (*   intros. *)
+    (*   invert  *)
+
+    Lemma adv_step_stays_in_R :
+      forall {A B} (U__i : IdealWorld.universe A) (U__r : universe A B) (R : universe A B -> IdealWorld.universe A -> Prop)
+              (cmd : user_cmd B) lbl u_id userData (usrs : honest_users A) (adv : adversaries B) cs ks qmsgs,
+        U__r.(adversary) $? u_id = Some userData
+        -> (forall u_id', u_id' <> u_id -> U__r.(adversary) $? u_id' = None) (* single adversary *)
+        -> step_user u_id lbl
+                    (build_data_step U__r userData)
+                    (usrs, adv, cs, ks, qmsgs, cmd)
+        -> R (strip_adversary U__r) U__i
+        -> R (strip_adversary (buildUniverseAdv usrs adv cs u_id {| key_heap := ks; protocol := cmd; msg_heap := qmsgs |})) U__i.
+    Proof.
+      intros.
+
+      pose proof H1 as STEP.
+      unfold build_data_step in STEP.
+      eapply adv_step_implies_no_new_ciphers_after_cleaning in STEP; eauto.
+
+      unfold buildUniverseAdv, strip_adversary, updateUserList in *; simpl in *.
+
+      assert (U__r.(adversary) = $0 $+ (u_id,userData)).
+      apply map_eq_Equal; unfold Equal; intros.
+      case (y ==n u_id); intro.
+      subst. rewrite H. rewrite add_eq_o by trivial; trivial.
+      specialize (H0 _ n). rewrite H0. rewrite add_neq_o by auto. eauto.
+
+      assert (findUserKeys U__r.(adversary) = userData.(key_heap)).
+      rewrite H3; unfold findUserKeys, fold, Raw.fold; simpl; rewrite empty_add_idempotent; trivial.
+
+      rewrite H4 in H2; rewrite STEP in H2.
+
+      assert (findUserKeys (adv $+ (u_id, {| key_heap := ks; protocol := cmd; msg_heap := qmsgs |})) = ks).
+      pose proof H1 as NOADD; unfold build_data_step in NOADD.
+
+      (* eapply user_step_adds_removes_no_adversaries in NOADD. *)
+      (* unfold iff in NOADD; invert NOADD. *)
+
+      assert (adv $+ (u_id, {| key_heap := ks; protocol := cmd; msg_heap := qmsgs |}) = $0 $+ (u_id, {| key_heap := ks; protocol := cmd; msg_heap := qmsgs |})).
+      apply map_eq_Equal; unfold Equal; intros.
+      case (y ==n u_id); intros.
+      subst; do 2 rewrite add_eq_o by trivial; trivial.
+      do 2 rewrite add_neq_o by auto; simpl. specialize (H0 _ n).
+      eapply user_step_adds_removes_no_adversaries with (u_id' := y) in NOADD; eauto.
+      unfold iff in NOADD; invert NOADD.
+      case_eq (adv $? y); intros.
+      assert (adv $? y <> None). unfold not; intro. rewrite H7 in H8. invert H8.
+      assert (adversary U__r $? u_id <> None); unfold not. intro. rewrite H9 in H; invert H.
+      admit.
+      rewrite empty_o; trivial.
+      rewrite H5. unfold findUserKeys.
+      rewrite fold_add; eauto.
+      simpl. unfold fold, Raw.fold; simpl. rewrite empty_add_idempotent. eauto.
+
+      admit. admit. admit.
+
+      rewrite H5. admit.
+
+    Admitted.
+
 
   End RealWorldLemmas.
 
@@ -241,6 +598,7 @@ Section SingleAdversarySimulates.
     end.
   Hint Extern 1 (_ = RealWorld.adversary _) => solve [ symmetry ; assumption ].
 
+
   Lemma simulates_with_adversary_silent :
     forall {A B} (U__ra : RealWorld.universe A B) (U__i : IdealWorld.universe A) (R : RealWorld.universe A B -> IdealWorld.universe A -> Prop),
       (forall (U__r : RealWorld.universe A B) (U__i : IdealWorld.universe A),
@@ -268,27 +626,19 @@ Section SingleAdversarySimulates.
                                                             {| RealWorld.key_heap := ks
                                                              ; RealWorld.protocol := cmd
                                                              ; RealWorld.msg_heap := qmsgs |})) ).
-      eapply RealWorld.StepUser; eauto. eapply honest_step_advuniv_implies_honest_step_origuniv; eauto.
+      eapply RealWorld.StepUser; eauto.
+      eapply honest_step_advuniv_implies_honest_step_origuniv; eauto.
       smash_universe.
+      unfold strip_adversary; smash_universe.
+      simpl. admit.
 
-      specialize (H _ _ H0 _ UNIV_STEP); eauto.
+      eapply H; eauto.
 
-      (* Adversary step *)
-    - invert H3; unfold RealWorld.build_data_step; simpl; [
-        | unfold strip_adversary, RealWorld.buildUniverseAdv, updateUserList;
-            simpl;
-            exists U__i;
-            match goal with | [ H : R (strip_adversary _) _ |- _ ] => progress unfold strip_adversary in H; simpl in H end;
-            intuition ..
-      ].
-
-      + admit.
-      + (* send *)
-        admit.
-      + (* enc *)
-        admit.
-      + (* sign *)
-        admit.
+    - exists U__i. constructor.
+      eapply TrcRefl.
+      eapply adv_step_stays_in_R; eauto.
+      intros.
+      admit. (* single adversary assumption *)
 
   Admitted.
 
@@ -315,7 +665,7 @@ Section SingleAdversarySimulates.
   Proof.
     simpl.
     intros.
-    invert H1.
+    invert H1. 
 
     assert (UNIV_STEP :
               RealWorld.step_universe
@@ -326,9 +676,10 @@ Section SingleAdversarySimulates.
                                                              ; RealWorld.protocol := cmd
                                                              ; RealWorld.msg_heap := qmsgs |})) ).
 
-    eapply RealWorld.StepUser. exact H2.
-    eapply honest_step_advuniv_implies_honest_step_origuniv; eauto.
-    smash_universe.
+    eapply RealWorld.StepUser; eauto.
+    eapply honest_step_advuniv_implies_honest_step_origuniv; simpl; eauto.
+    unfold strip_adversary; simpl; smash_universe. simpl.
+    admit.
 
     specialize (H _ _ H0 _ _ UNIV_STEP).
 
@@ -344,6 +695,19 @@ Section SingleAdversarySimulates.
 
   Admitted.
 
+  Lemma fun_cipher_match :
+    (fun (k : key) (v : RealWorld.cipher) (m : t RealWorld.cipher) =>
+       if match v with
+          | RealWorld.Cipher _ _ _ => true
+          end then m $+ (k, v) else m)
+      = 
+    (fun (k : key) (v : RealWorld.cipher) (m : t RealWorld.cipher) =>
+       m $+ (k, v)).
+  Proof.
+    simpl.
+    (* rewrite cipher_is_Cipher. *)
+  Admitted.
+      
   Theorem simulates_ok_with_adversary :
     forall {A B} (U__r : RealWorld.universe A B) (U__i : IdealWorld.universe A),
       U__r <| U__i
@@ -361,9 +725,12 @@ Section SingleAdversarySimulates.
     exists (fun ur ui => R (strip_adversary ur) ui); unfold simulates.
     propositional;
       eauto using simulates_with_adversary_silent, simulates_with_adversary_loud.
-    - rewrite H1;
-        unfold strip_adversary, add_adversary; simpl;
-          rewrite <- H0; rewrite univ_components; eauto.
+    - rewrite H1; unfold strip_adversary, add_adversary; simpl.
+      rewrite H0. rewrite empty_add_idempotent.
+      unfold RealWorld.findUserKeys, fold; simpl. rewrite empty_add_idempotent.
+
+      unfold clean_ciphers, honest_cipher; simpl. rewrite fun_cipher_match; simpl. rewrite fold_over_empty. simpl.
+      rewrite <- H0; rewrite univ_components. auto.
   Qed.
 
 End SingleAdversarySimulates.
